backends/lean/Aeneas/Data/ListN.lean
@@ -1,0 +1,34 @@
+namespace Aeneas.Data.ListN
+
+inductive ListN.{u} (α : Type u) : Nat → Type u where
+| nil : ListN α 0
+| cons {n} : α → ListN α n → ListN α n.succ
+deriving BEq, ReflBEq, LawfulBEq, DecidableEq
+
+def ListN.toList {a n} (l : ListN a n) : List a :=
+  match l with
+  | .nil => .nil
+  | .cons a l' => .cons a l'.toList
+
+def ListN.fromList {a} (l : List a) : ListN a l.length :=
+  match l with
+  | .nil => .nil
+  | .cons a l' => .cons a (ListN.fromList l')
+
+theorem ListN.from_to_inverse {α} {l : List α}: (ListN.fromList l).toList = l := by
+  induction l <;> grind [toList, fromList]
+
+theorem ListN_length {α n} (l : ListN α n) : l.toList.length = n := by
+  induction l <;> grind [ListN.toList]
+
+theorem ListN.to_from_inverse {α n} {l : ListN α n}
+  : ListN.fromList l.toList ≍ l := by
+  induction l <;> simp [toList, fromList]
+  rename_i n a l ih
+  congr -- TODO: how does this tactic work here?
+  apply ListN_length
+
+theorem ListN.toList_inj {α n} (l1 l2 : ListN α n) (h : l1.toList = l2.toList) : l1 = l2 := by
+  induction l1 <;> cases l2 <;> grind [ListN.toList]
+
+end Aeneas.Data.ListN
